Packing: add all functions

Clap/Packing.lean
@@ -21,6 +21,88 @@ def assertIsBytes [Fact (Primes.fits p 8)] {numBytes : ℕ}
   _ ← a.mapM F8.ofF!
   pure ()
 
+def num2BigEndianBits (w : ℕ) (x : F p) : Option (FBitVec p) := do
+  let bits ← num2bits w x
+  pure bits.reverse
+
+def bigEndianBits2Num : FBitVec p → F p := bits2num ∘ .reverse
+
+def bytes2BigEndianBits {n : ℕ} (bytes : Vector (F p) n) : Option (FBitVec p) := do
+  let bits ← bytes.mapM (num2BigEndianBits 8)
+  return bits.foldl .append []
+
+def chunksToFieldElem {numChuncks : ℕ}
+  (bitsPerChunk : ℕ)
+  (chunks : Vector (F p) numChuncks) :
+  Option (F p)
+:= do
+  if ¬Primes.fits p (numChuncks * bitsPerChunk) then .none
+  let base := 2^bitsPerChunk
+  return chunks.reverse.foldl (fun acc x ↦ acc * base + x) 0
+
+-- TODO (Andrei): Decide if `chunks` should be List or Vector.
+def chunksToFieldElem' (numChuncks : ℕ)
+  (bitsPerChunk : ℕ)
+  (chunks : List (F p)) :
+  Option (F p)
+:= do
+  if ¬Primes.fits p (numChuncks * bitsPerChunk) then .none
+  let base := 2^bitsPerChunk
+  return chunks.reverse.foldl (fun acc x ↦ acc * base + x) 0
+
+def bigEndianBitsToScalars
+  (bitsPerScalar : ℕ)
+  (bits : FBitVec p) :
+  Option (Array (F p))
+:= do
+  if ¬Primes.fits p bitsPerScalar then .none
+  if h : 0 < bitsPerScalar then
+    step bitsPerScalar h bits .empty
+  else
+    .none
+ where
+  step (bitsPerScalar : ℕ) (h₁ : 0 < bitsPerScalar)
+    (bits : FBitVec p)
+    (acc : Array (F p)) :
+    Array (F p)
+  :=
+    if h₂ : bits.isEmpty then acc else
+      let x := bits.take bitsPerScalar
+      let x := bigEndianBits2Num x
+      have : 0 < bits.length := by
+        simp [List.isEmpty_iff] at h₂
+        simp only [← Nat.ne_zero_iff_zero_lt, ne_eq, List.length_eq_zero_iff]
+        exact h₂
+      step bitsPerScalar h₁ (bits.drop bitsPerScalar) (acc.push x)
+  termination_by bits.length
+
+-- TODO (Andrei): Decide if `chunks` should be List or Vector.
+def chunksToFieldElems {numChuncks : ℕ}
+  (chunksPerScalar bitsPerChunk : ℕ)
+  (chunks : Vector (F p) numChuncks) :
+  Option (Array (F p))
+:= do
+  if numChuncks == 0 then .none
+  if h : 0 < chunksPerScalar then
+    step chunksPerScalar h chunks.toArray.toList .empty
+  else
+    .none
+ where
+  step (chunksPerScalar : ℕ) (h₁ : 0 < chunksPerScalar)
+    (bits : List (F p))
+    (acc : Array (F p)) :
+    Option (Array (F p))
+  :=
+    if h₂ : bits.isEmpty then acc else do
+      let x := bits.take chunksPerScalar
+      let x ← chunksToFieldElem' numChuncks bitsPerChunk x
+      have : 0 < bits.length := by
+        simp [List.isEmpty_iff] at h₂
+        simp only [← Nat.ne_zero_iff_zero_lt, ne_eq, List.length_eq_zero_iff]
+        exact h₂
+      step chunksPerScalar h₁ (bits.drop chunksPerScalar) (acc.push x)
+  termination_by bits.length
+
 end Packing
 
 namespace TestPacking
@@ -30,14 +112,66 @@ open Clap.Lang Core ZMod
 
 abbrev p := Primes.bn254
 
-example : assertIs64BitLimbs (p := p) (#v[1, 2, 3, 4]) = .some () := by native_decide
-example : assertIs64BitLimbs (p := p) (#v[1, 2, 3, 2^64-1]) = .some () := by native_decide
-example : assertIs64BitLimbs (p := p) (#v[2^64]) = .none := by native_decide
-example : assertIs64BitLimbs (p := p) (#v[1, 2, 2^64 + 5]) = .none := by native_decide
+example : assertIs64BitLimbs (p := p) #v[1, 2, 3, 4] = .some () := by native_decide
+example : assertIs64BitLimbs (p := p) #v[1, 2, 3, 2^64-1] = .some () := by native_decide
+example : assertIs64BitLimbs (p := p) #v[2^64] = .none := by native_decide
+example : assertIs64BitLimbs (p := p) #v[1, 2, 2^64+5] = .none := by native_decide
 
-example : assertIsBytes (p := p) (#v[1, 2, 3, 4]) = .some () := by native_decide
-example : assertIsBytes (p := p) (#v[1, 2, 3, 2^8-1]) = .some () := by native_decide
-example : assertIsBytes (p := p) (#v[2^8]) = .none := by native_decide
-example : assertIsBytes (p := p) (#v[1, 2, 2^8  + 5]) = .none := by native_decide
+example : assertIsBytes (p := p) #v[1, 2, 3, 4] = .some () := by native_decide
+example : assertIsBytes (p := p) #v[1, 2, 3, 2^8-1] = .some () := by native_decide
+example : assertIsBytes (p := p) #v[2^8] = .none := by native_decide
+example : assertIsBytes (p := p) #v[1, 2, 2^8+5] = .none := by native_decide
+
+example : num2BigEndianBits (p := p) 3 6 = .some [1, 1, 0] := by native_decide
+example : num2BigEndianBits (p := p) 3 1 = .some [0, 0, 1] := by native_decide
+example : num2BigEndianBits (p := p) 3 8 = .none := by native_decide
+example : num2BigEndianBits (p := p) 0 0 = .some [] := by native_decide
+example : num2BigEndianBits (p := p) 0 1 = .none := by native_decide
+
+example : bigEndianBits2Num (p := p) [] = 0 := by rfl
+example : bigEndianBits2Num (p := p) [0] = 0 := by rfl
+example : bigEndianBits2Num (p := p) [1, 1, 0, 0] = 12 := by rfl
+
+example :
+  bytes2BigEndianBits (p := p) #v[] = .some []
+:= by native_decide
+example :
+  bytes2BigEndianBits (p := p) #v[1] = .some [0, 0, 0, 0, 0, 0, 0, 1]
+:= by native_decide
+example :
+  bytes2BigEndianBits (p := p) #v[2^8-1, 1] =
+    .some [1, 1, 1, 1, 1, 1, 1, 1, 0, 0, 0, 0, 0, 0, 0, 1]
+:= by
+  native_decide
+example :
+  bytes2BigEndianBits (p := p) #v[2^8] = .none
+:= by
+  native_decide
+
+example : chunksToFieldElem (p := p) 2 #v[] = .some 0 := by rfl
+/-- [00₂, 11₂, 10₂] -> 101100₂ -/
+example : chunksToFieldElem (p := p) 2 #v[0, 3, 2] = .some 44 := by native_decide
+/-- Doesn't fit -/
+example : chunksToFieldElem (p := p) (p.log2 + 1) #v[1] = .none := by rfl
+/-- [00₂, 11₂, 10₂, 01₂, 11₂, 10₂] -> 101100₂, 101101₂ -/
+
+example : chunksToFieldElems (p := p) 3 2 #v[0,3,2, 1,3,2] = .some #[44, 45] := by
+  native_decide
+example :
+  chunksToFieldElems (p := p) 1 2 #v[0, 3, 2, 1, 3, 2] =.some #[0, 3, 2, 1, 3, 2]
+:= by native_decide
+example : chunksToFieldElems (p := p) 0 2 #v[0, 3, 2, 1, 3, 2] = .none := by native_decide
+example : chunksToFieldElems (p := p) 3 1 #v[0, 1, 1, 1, 0, 0] = some #[6, 1] := by native_decide
+example : chunksToFieldElems (p := p) 3 1 #v[0, 1, 1, 1] = some #[6, 1] := by native_decide
+
+example :
+  bigEndianBitsToScalars (p := p) 4 [0,0,0,0, 0,0,0,1, 0,1,1] = .some #[0, 1, 3]
+:= by native_decide
+example :
+  bigEndianBitsToScalars (p := p) 4 [0,0,0,0, 0,0,0,1, 0,1,1,0] = .some #[0, 1, 6]
+:= by native_decide
+example :
+  bigEndianBitsToScalars (p := p) 0 [0,0,0,0, 0,0,0,1, 0,1,1,0] = .none
+:= by native_decide
 
 end TestPacking
